src/casemate-check-rocq/theories/utils.v
@@ -125,7 +125,7 @@ Inductive sm_owner_t :=
 Global Instance owner_t_eq_decision : EqDecision sm_owner_t.
   Proof. solve_decision. Qed.
 
-Definition root_val (root : sm_owner_t) : phys_addr_t :=
+Definition owner_val (root : sm_owner_t) : phys_addr_t :=
   match root with
   | Root r => r
   end
@@ -141,9 +141,11 @@ Inductive vmid_t :=
  .
 
 Inductive addr_id_t :=
-  | ASID : u64 -> addr_id_t
-  | VMID : u64 -> addr_id_t
+  | AID : u64 -> addr_id_t
 .
+
+Global Instance addr_id_t_eq_decision : EqDecision addr_id_t.
+  Proof. solve_decision. Qed.
 
 Inductive result (A B: Type): Type :=
   | Ok (a: A)
